examples/Proc.v
@@ -7,8 +7,15 @@ Inductive term : Set :=
 | tend : term
 | tfix : term -> term
 | tact : action -> term -> term
-| tpar : term -> term -> term (* parallel *)
-| tbra : term -> term -> term (* branching *)
+
+(* parallel *)
+| tpar : term -> term -> term
+
+(* active selection/branching *)
+(* | tbra : term -> term -> term  *)
+
+(* passive option selection/branching *)
+(* | topt : term -> term -> term  *)
 .
 
 Fixpoint tsubst (t1 : term) (t2 : term) :=
@@ -18,7 +25,8 @@ Fixpoint tsubst (t1 : term) (t2 : term) :=
   | tfix t => tfix t
   | tact a t => tact a (tsubst t1 t)
   | tpar tl tr => tpar (tsubst t1 tl) (tsubst t1 tr)
-  | tbra tl tr => tbra (tsubst t1 tl) (tsubst t1 tr)
+  (* | tbra tl tr => tbra (tsubst t1 tl) (tsubst t1 tr) *)
+  (* | topt tl tr => topt (tsubst t1 tl) (tsubst t1 tr) *)
   end.
 
 (* true: "comm", false: "silent" *)
@@ -37,45 +45,55 @@ Inductive termLTS : term -> bool -> term -> Prop :=
     termLTS (tpar (tact CSend tl) (tact CRecv tr))
       true  (tpar tl tr)
 
-(* non-deterministic choice between tl and tr *)
-| do_bral : forall a tl tr tl',                     (* 3*)
-    termLTS tl a tl' ->
-    termLTS (tbra tl tr) a tl'
-
-| do_brar : forall a tl tr tr',                     (* 4*)
-    termLTS tr a tr' ->
-    termLTS (tbra tl tr) a tr'
-
 (* non-deterministic parallel step *)
-| do_parl : forall a tl tl' tr,                     (* 5*)
+| do_parl : forall a tl tl' tr,                     (* 3*)
     termLTS tl a tl' ->
     termLTS (tpar tl tr) a (tpar tl' tr)
 
-| do_parr : forall a tl tr tr',                     (* 6*)
+| do_parr : forall a tl tr tr',                     (* 4*)
     termLTS tr a tr' ->
     termLTS (tpar tl tr) a (tpar tl tr')
 
 (* These below capture "structural congruence": using "silent" transitions *)
-| do_fix : forall t,                                (* 7*)
+| do_fix : forall t,                                (* 5*)
     termLTS (tfix t) false (tsubst (tfix t) t)
 
-| do_comm : forall tl tr,                           (* 8*)
+| do_comm : forall tl tr,                           (* 6*)
     termLTS (tpar tl tr) false (tpar tr tl)
 
-| do_assocl : forall t1 t2 t3,                      (* 9*)
+| do_assocl : forall t1 t2 t3,                      (* 7*)
     termLTS (tpar t1 (tpar t2 t3)) false (tpar (tpar t1 t2) t3)
 
-| do_assocr : forall t1 t2 t3,                      (*10*)
+| do_assocr : forall t1 t2 t3,                      (* 8*)
     termLTS (tpar (tpar t1 t2) t3) false (tpar t1 (tpar t2 t3))
 
+(* non-deterministic selection between tl and tr *)
+(* | do_bral : forall a tl tr tl',                     (* 9*)
+    termLTS tl a tl' ->
+    termLTS (tbra tl tr) a tl'
+
+| do_brar : forall a tl tr tr',                     (*10*)
+    termLTS tr a tr' ->
+    termLTS (tbra tl tr) a tr' *)
+
+(* non-deterministic branch in reaction to ready party p *)
+(* | do_optl : forall tl tr p c,                       (*11*)
+    termLTS (tpar p tl) true c ->
+    termLTS (tpar p (topt tl tr)) true c
+
+| do_optr : forall tl tr p c,                       (*12*)
+    termLTS (tpar p tr) true c ->
+    termLTS (tpar p (topt tl tr)) true c *)
+
+
 (* Below are attempts to "clean up" recursive terms. *)
-(* | do_clean :                                        (*11*)
+(* | do_clean :                                        (*13*)
     termLTS (tpar tend tend) false tend
 
-| do_clean_l : forall tr,                           (*12*)
+| do_clean_l : forall tr,                           (*14*)
     termLTS (tpar tend tr) false tr
 
-| do_clean_r : forall tl,                           (*13*)
+| do_clean_r : forall tl,                           (*15*)
     termLTS (tpar tl tend) false tl *)
 .
 
@@ -95,6 +113,7 @@ Inductive transitive_closure : term -> Prop :=
 Example proc0_send0 := tact ASend tend. (* empty lts *)
 (* MeBi Show LTS Bounded 150 Of proc0_send0 Using termLTS. *)
 
+
 Example proc0_send1a := tpar (tact ASend tend)
                              (tact ARecv tend).
 (* MeBi Show LTS Bounded 150 Of proc0_send1a Using termLTS. *)
@@ -108,25 +127,29 @@ Goal transitive_closure proc0_send1a.
   constructor.
 Qed.
 
+
 Example proc0_send1b := tpar (tact ARecv tend)
                              (tact ASend tend).
 (* MeBi Show LTS Bounded 150 Of proc0_send1a Using termLTS. *)
+
 
 Example proc0_send2 := tpar (tact ASend (tact ARecv tend))
                             (tact ARecv (tact ASend tend)).
 (* MeBi Show LTS Bounded 150 Of proc0_send2 Using termLTS. *)
 
-Goal transitive_closure proc0_send2.
+(* Goal transitive_closure proc0_send2.
   unfold proc0_send2.
   eapply trans_step. apply do_senda.
   eapply trans_step. apply do_comm.
   eapply trans_step. apply do_senda.
   constructor.
-Qed.
+Qed. *)
+
 
 Example proc0_send3 := tpar (tact ASend (tact BSend tend))
                             (tact ARecv (tact BRecv tend)).
 (* MeBi Show LTS Bounded 150 Of proc0_send3 Using termLTS. *)
+
 
 Example proc0_send4 := tpar (tact BSend (tact ARecv tend))
                             (tact BRecv (tact ASend tend)).
@@ -135,22 +158,25 @@ Example proc0_send4 := tpar (tact BSend (tact ARecv tend))
 
 
 (*************************************)
-(** Simple Recursion, no Branching ***)
+(** Recursion ************************)
 (*************************************)
 
 Example proc1_rec1 := tfix trec.
 (* MeBi Show LTS Bounded 150 Of proc1_rec1 Using termLTS. *)
 (* MeBi Dump "proc1_rec1" LTS Bounded 150 Of proc1_rec1 Using termLTS. *)
 
+
 Example proc1_rec2 := tpar (tfix (tact ASend trec))
                            (tfix (tact ARecv trec)).
 (* MeBi Show LTS Bounded 150 Of proc1_rec2 Using termLTS. *)
 (* MeBi Dump "proc1_rec2" LTS Bounded 150 Of proc1_rec2 Using termLTS. *)
 
+
 Example proc1_rec3 := tpar (tfix (tact ASend (tact BSend trec)))
                            (tfix (tact ARecv (tact BRecv trec))).
 (* MeBi Show LTS Bounded 150 Of proc1_rec3 Using termLTS. *)
 (* MeBi Dump "proc1_rec3" LTS Bounded 150 Of proc1_rec3 Using termLTS. *)
+
 
 Example proc1_rec4 := tpar (tact ASend (tfix (tact BSend trec)))
                            (tact ARecv (tfix (tact BRecv trec))).
@@ -158,99 +184,283 @@ Example proc1_rec4 := tpar (tact ASend (tfix (tact BSend trec)))
 (* MeBi Dump "proc1_rec4" LTS Bounded 150 Of proc1_rec4 Using termLTS. *)
 
 
+Example proc1_rec5 := tpar (tfix (tact ASend (tact ASend trec)))
+                           (tfix (tact ARecv trec)).
+(* MeBi Show LTS Bounded 150 Of proc1_rec5 Using termLTS. *)
+MeBi Dump "proc1_rec5" LTS Bounded 150 Of proc1_rec5 Using termLTS.
+
+
+Example proc1_rec6 := tpar (tact ASend (tact BSend (tfix (tact ASend trec))))
+                           (tpar (tfix (tact ARecv trec))
+                                 (tact BSend tend)).
+(* MeBi Show LTS Bounded 150 Of proc1_rec6 Using termLTS. *)
+MeBi Dump "proc1_rec6" LTS Bounded 150 Of proc1_rec6 Using termLTS.
+
+
+(* FIXME: grows forever by accumulating [tend]. (need structural equiv.) *)
+Example proc1_rec7 := tfix (tpar (tact ASend (tact BSend trec))
+                                 (tact ARecv (tact BRecv tend))).
+(* MeBi Show LTS Bounded 150 Of proc1_rec7 Using termLTS. *)
+MeBi Dump "proc1_rec7" LTS Bounded 150 Of proc1_rec7 Using termLTS.
+
+
+
+
+
+
+(****************************************************************************)
+(** Layered Semantics *******************************************************)
+(****************************************************************************)
+
+Inductive comp : Set :=
+| cterm : term -> comp
+| cpar : comp -> comp -> comp
+.
+
+Inductive compLTS : comp -> bool -> comp -> Prop :=
+| do_t : forall a t t',
+    termLTS t a t' ->
+    compLTS (cterm t) a (cterm t')
+
+| do_l : forall a l l' r,
+    compLTS l a l' ->
+    compLTS (cpar l r) a (cpar l' r)
+
+| do_r : forall a l r r',
+    compLTS r a r' ->
+    compLTS (cpar l r) a (cpar l r')
+
+| do_l_end : forall a r,
+    compLTS (cpar (cterm tend) r) a r
+
+| do_r_end : forall a l,
+    compLTS (cpar l (cterm tend)) a l
+.
+
+(*************************************)
+(** Basic: No recursion or branches **)
+(*************************************)
+
+Example comp1_rec1 := cpar (cterm proc1_rec1) (cterm proc1_rec1).
+(* MeBi Show LTS Bounded 150 Of comp0_send1 Using termLTS compLTS. *)
+MeBi Dump "comp1_rec1" LTS Bounded 350 Of comp1_rec1 Using termLTS compLTS.
+
+(*************************************)
+(** Recursion ************************)
+(*************************************)
+
+Example comp0_send1 := cpar (cterm proc0_send1a) (cterm proc0_send1b).
+(* MeBi Show LTS Bounded 150 Of comp1_rec1 Using termLTS compLTS. *)
+MeBi Dump "comp0_send1" LTS Bounded 350 Of comp0_send1 Using termLTS compLTS.
+
+
+
+
+
+
+(****************************************************************************)
+(** Problematic Terms (Branching) *******************************************)
+(** (Requires [tbra] and [topt] ) *******************************************)
+(****************************************************************************)
+(** Issues arise with branching AND recursion *******************************)
+(****************************************************************************)
+
+
+Inductive bad_term : Set :=
+| bad_trec : bad_term
+| bad_tend : bad_term
+| bad_tfix : bad_term -> bad_term
+| bad_tact : action -> bad_term -> bad_term
+
+(* parallel *)
+| bad_tpar : bad_term -> bad_term -> bad_term
+
+(* active selection/branching *)
+| bad_tbra : bad_term -> bad_term -> bad_term
+
+(* passive option selection/branching *)
+| bad_topt : bad_term -> bad_term -> bad_term
+.
+
+Fixpoint bad_tsubst (t1 : bad_term) (t2 : bad_term) :=
+  match t2 with
+  | bad_trec => t1
+  | bad_tend => bad_tend
+  | bad_tfix t => bad_tfix t
+  | bad_tact a t => bad_tact a (bad_tsubst t1 t)
+  | bad_tpar tl tr => bad_tpar (bad_tsubst t1 tl) (bad_tsubst t1 tr)
+  | bad_tbra tl tr => bad_tbra (bad_tsubst t1 tl) (bad_tsubst t1 tr)
+  | bad_topt tl tr => bad_topt (bad_tsubst t1 tl) (bad_tsubst t1 tr)
+  end.
+
+(* true: "comm", false: "silent" *)
+Inductive bad_termLTS : bad_term -> bool -> bad_term -> Prop :=
+(* syncrhonous communication, i.e., send/recv in parallel *)
+
+| bad_do_senda : forall tl tr,                          (* 0*)
+    bad_termLTS (bad_tpar (bad_tact ASend tl) (bad_tact ARecv tr))
+      true  (bad_tpar tl tr)
+
+| bad_do_sendb : forall tl tr,                          (* 1*)
+    bad_termLTS (bad_tpar (bad_tact BSend tl) (bad_tact BRecv tr))
+      true  (bad_tpar tl tr)
+
+| bad_do_sendc : forall tl tr,                          (* 2*)
+    bad_termLTS (bad_tpar (bad_tact CSend tl) (bad_tact CRecv tr))
+      true  (bad_tpar tl tr)
+
+(* non-deterministic parallel step *)
+| bad_do_parl : forall a tl tl' tr,                     (* 3*)
+    bad_termLTS tl a tl' ->
+    bad_termLTS (bad_tpar tl tr) a (bad_tpar tl' tr)
+
+| bad_do_parr : forall a tl tr tr',                     (* 4*)
+    bad_termLTS tr a tr' ->
+    bad_termLTS (bad_tpar tl tr) a (bad_tpar tl tr')
+
+(* These below capture "structural congruence": using "silent" transitions *)
+| bad_do_fix : forall t,                                (* 5*)
+    bad_termLTS (bad_tfix t) false (bad_tsubst (bad_tfix t) t)
+
+| bad_do_comm : forall tl tr,                           (* 6*)
+    bad_termLTS (bad_tpar tl tr) false (bad_tpar tr tl)
+
+| bad_do_assocl : forall t1 t2 t3,                      (* 7*)
+    bad_termLTS (bad_tpar t1 (bad_tpar t2 t3)) false (bad_tpar (bad_tpar t1 t2) t3)
+
+| bad_do_assocr : forall t1 t2 t3,                      (* 8*)
+    bad_termLTS (bad_tpar (bad_tpar t1 t2) t3) false (bad_tpar t1 (bad_tpar t2 t3))
+
+(* non-deterministic selection between tl and tr *)
+| bad_do_bral : forall a tl tr tl',                     (* 9*)
+    bad_termLTS tl a tl' ->
+    bad_termLTS (bad_tbra tl tr) a tl'
+
+| bad_do_brar : forall a tl tr tr',                     (*10*)
+    bad_termLTS tr a tr' ->
+    bad_termLTS (bad_tbra tl tr) a tr'
+
+(* non-deterministic branch in reaction to ready party p *)
+| bad_do_optl : forall tl tr p c,                       (*11*)
+    bad_termLTS (bad_tpar p tl) true c ->
+    bad_termLTS (bad_tpar p (bad_topt tl tr)) true c
+
+| bad_do_optr : forall tl tr p c,                       (*12*)
+    bad_termLTS (bad_tpar p tr) true c ->
+    bad_termLTS (bad_tpar p (bad_topt tl tr)) true c
+
+
+(* Below are attempts to "clean up" recursive terms. *)
+(* | bad_do_clean :                                        (*13*)
+    bad_termLTS (bad_tpar bad_tend bad_tend) false bad_tend
+
+| bad_do_clean_l : forall tr,                           (*14*)
+    bad_termLTS (bad_tpar bad_tend tr) false tr
+
+| bad_do_clean_r : forall tl,                           (*15*)
+    bad_termLTS (bad_tpar tl bad_tend) false tl *)
+.
+
+
 (*************************************)
 (** Branching, no Recursion **********)
 (*************************************)
 
-(** the example below does nothing since neither branch can occur *)
-(* Example proc2_bra1 := tpar (tbra (tact ASend tend)
-                                 (tact BSend tend))
-                           (tbra (tact ARecv tend)
-                                 (tact BRecv tend)).
-(* MeBi Show LTS Bounded 150 Of proc2_bra1 Using termLTS. *)
-MeBi Dump "proc2_bra1" LTS Bounded 150 Of proc2_bra1 Using termLTS. *)
+Example proc2_bra1 := bad_tbra (bad_tpar (bad_tact ASend bad_tend)
+                                         (bad_tact ARecv bad_tend))
+                               (bad_tpar (bad_tact BSend bad_tend)
+                                         (bad_tact BRecv bad_tend)).
+(* MeBi Show LTS Bounded 150 Of proc2_bra1 Using bad_termLTS. *)
+MeBi Dump "proc2_bra1" LTS Bounded 150 Of proc2_bra1 Using bad_termLTS.
 
-Example proc2_bra2 := tbra (tpar (tact ASend tend)
-                                 (tact ARecv tend))
-                           (tpar (tact BSend tend)
-                                 (tact BRecv tend)).
-(* MeBi Show LTS Bounded 150 Of proc2_bra2 Using termLTS. *)
-(* MeBi Dump "proc2_bra2" LTS Bounded 150 Of proc2_bra2 Using termLTS. *)
+Example proc2_bra2 :=
+    bad_tbra (bad_tpar (bad_tact ASend (bad_tact BSend bad_tend))
+                       (bad_tact ARecv (bad_tact BRecv bad_tend)))
+             (bad_tpar (bad_tact BSend (bad_tact ASend bad_tend))
+                       (bad_tact BRecv (bad_tact ARecv bad_tend))).
+(* MeBi Show LTS Bounded 150 Of proc2_bra2 Using bad_termLTS. *)
+MeBi Dump "proc2_bra2" LTS Bounded 150 Of proc2_bra2 Using bad_termLTS.
 
-Example proc2_bra3 := tbra (tpar (tact ASend (tact BSend tend))
-                                 (tact ARecv (tact BRecv tend)))
-                           (tpar (tact BSend (tact ASend tend))
-                                 (tact BRecv (tact ARecv tend))).
-(* MeBi Show LTS Bounded 150 Of proc2_bra3 Using termLTS. *)
-(* MeBi Dump "proc2_bra3" LTS Bounded 150 Of proc2_bra3 Using termLTS. *)
-
-Example proc2_bra4 := tbra (tpar (tact ASend (tact BSend tend))
-                                 (tact ARecv (tact BRecv tend)))
-                           (tbra (tpar (tact BSend (tact CSend tend))
-                                       (tact BRecv (tact CRecv tend)))
-                                 (tpar (tact CSend (tact ASend tend))
-                                       (tact CRecv (tact ARecv tend)))).
-(* MeBi Show LTS Bounded 150 Of proc2_bra4 Using termLTS. *)
-(* MeBi Dump "proc2_bra4" LTS Bounded 150 Of proc2_bra4 Using termLTS. *)
-
-(** the example below does nothing since neither branch can occur *)
-(* Example proc2_bra5 := tpar (tact ARecv (tact BRecv tend))
-                           (tbra (tact ASend (tact BSend tend))
-                                 (tact BSend (tact ASend tend))).
-(* MeBi Show LTS Bounded 150 Of proc2_bra5 Using termLTS. *)
-MeBi Dump "proc2_bra5" LTS Bounded 150 Of proc2_bra5 Using termLTS. *)
+Example proc2_bra3 :=
+    bad_tbra (bad_tpar (bad_tact ASend (bad_tact BSend bad_tend))
+                       (bad_tact ARecv (bad_tact BRecv bad_tend)))
+             (bad_tbra (bad_tpar (bad_tact BSend (bad_tact CSend bad_tend))
+                                 (bad_tact BRecv (bad_tact CRecv bad_tend)))
+                       (bad_tpar (bad_tact CSend (bad_tact ASend bad_tend))
+                                 (bad_tact CRecv (bad_tact ARecv bad_tend)))).
+(* MeBi Show LTS Bounded 150 Of proc2_bra3 Using bad_termLTS. *)
+MeBi Dump "proc2_bra3" LTS Bounded 150 Of proc2_bra3 Using bad_termLTS.
 
 
 (*************************************)
 (** Simple Branching and Recursion ***)
 (*************************************)
 
-(* NOTE: the examples below caused a state explosion. This is partially due *)
-(* to their defintion, but also due to the [tend] and [tpar] not being      *)
-(* cleaned up. *)
-
-Example proc3_recbra1 := tfix (tbra (tpar (tact ASend trec)
-                                          (tact ARecv trec))
-                                    (tpar (tact BSend tend)
-                                          (tact BRecv tend))).
-(* MeBi Show LTS Bounded 1000 Of proc3_recbra1 Using termLTS. *)
-MeBi Dump "proc3_recbra1" LTS Bounded 1000 Of proc3_recbra1 Using termLTS.
-
-(* NOTE: duplicates start appearing at exactly 135 and onwards. *)
-(* MeBi Dump "proc3_recbra1" LTS Bounded 135 Of proc3_recbra1 Using termLTS. *)
+Example proc3_recbra1 :=
+    bad_tbra (bad_tfix (bad_tpar (bad_tact ASend bad_trec)
+                                 (bad_tact ARecv bad_trec)))
+             (bad_tpar (bad_tact BSend bad_tend)
+                       (bad_tact BRecv bad_tend)).
+(* MeBi Show LTS Bounded 1000 Of proc3_recbra1 Using bad_termLTS. *)
+MeBi Dump "proc3_recbra1" LTS Bounded 50 Of proc3_recbra1 Using bad_termLTS.
 
 
-(* NOTE: with the [do_clean] additions to the semantics, duplicates start appearing at exactly 120 and onwards. *)
-(* MeBi Dump "proc3_recbra1" LTS Bounded 120 Of proc3_recbra1 Using termLTS. *)
+Example proc3_recbra2 :=
+    bad_tfix (bad_tbra (bad_tpar (bad_tact ASend bad_trec)
+                                 (bad_tact ARecv bad_trec))
+                       (bad_tpar (bad_tact BSend bad_tend)
+                                 (bad_tact BRecv bad_tend))).
+(* MeBi Show LTS Bounded 1000 Of proc3_recbra2 Using bad_termLTS. *)
+(* MeBi Dump "proc3_recbra2" LTS Bounded 5000 Of proc3_recbra2 Using bad_termLTS. *)
 
-Example proc3_recbra2 := tfix (tbra (tpar (tact ASend trec)
-                                          (tact ARecv trec))
-                                    (tpar (tact BSend trec)
-                                          (tact BRecv trec))).
-(* MeBi Show LTS Bounded 1000 Of proc3_recbra2 Using termLTS. *)
-(* MeBi Dump "proc3_recbra2" LTS Bounded 2000 Of proc3_recbra2 Using termLTS. *)
 
-Example proc3_recbra3 := tbra (tfix (tpar (tact ASend trec)
-                                          (tact ARecv trec)))
-                              (tfix (tpar (tact BSend trec)
-                                          (tact BRecv trec))).
-(* MeBi Show LTS Bounded 1000 Of proc3_recbra3 Using termLTS. *)
-(* MeBi Dump "proc3_recbra3" LTS Bounded 2000 Of proc3_recbra3 Using termLTS. *)
+Example proc3_recbra3 :=
+    bad_tfix (bad_tbra (bad_tpar (bad_tact ASend bad_trec)
+                                 (bad_tact ARecv bad_trec))
+                       (bad_tpar (bad_tact BSend bad_trec)
+                                 (bad_tact BRecv bad_trec))).
+(* MeBi Show LTS Bounded 1000 Of proc3_recbra3 Using bad_termLTS. *)
+(* MeBi Dump "proc3_recbra3" LTS Bounded 2000 Of proc3_recbra3 Using bad_termLTS. *)
+
+Example proc3_recbra4 :=
+    bad_tbra (bad_tfix (bad_tpar (bad_tact ASend bad_trec)
+                                 (bad_tact ARecv bad_trec)))
+             (bad_tfix (bad_tpar (bad_tact BSend bad_trec)
+                                 (bad_tact BRecv bad_trec))).
+(* MeBi Show LTS Bounded 1000 Of proc3_recbra4 Using bad_termLTS. *)
+(* MeBi Dump "proc3_recbra4" LTS Bounded 2000 Of proc3_recbra4 Using bad_termLTS. *)
 
 (*************************************)
 (** Nested Branching and Recursion ***)
 (*************************************)
 
 
+(* the below example sends [ASend] and then [BSend]. *)
+Example proc1_nestedrec1 :=
+    bad_tfix (bad_tpar ((bad_tact ASend (bad_tact BSend bad_trec)))
+                       (bad_tfix (bad_topt (bad_tact ARecv bad_trec)
+                                           (bad_tact BRecv bad_tend)))).
+
+(* Goal transitive_closure proc1_nestedrec1.
+  unfold proc1_nestedrec1.
+  eapply trans_step. eapply do_fix. simpl.
+  eapply trans_step. eapply do_parr. eapply do_fix. simpl.
+  eapply trans_step. eapply do_optl. eapply do_senda.
+  eapply trans_step. eapply do_parr. eapply do_fix. simpl.
+  eapply trans_step. eapply do_optr. eapply do_sendb.
+  eapply trans_step. eapply do_clean_r.
+  constructor.
+Qed. *)
+
+(* MeBi Show LTS Bounded 150 Of proc1_nestedrec1 Using bad_termLTS. *)
+MeBi Dump "proc1_nestedrec1" LTS Bounded 50 Of proc1_nestedrec1 Using bad_termLTS.
 
 
-Example proc1 := tpar (tfix (tact ASend trec)) (tfix (tact ARecv trec)).
-(* MeBi Show LTS Bounded 150 Of proc1 Using termLTS. *)
-(* MeBi Dump "proc1" LTS Bounded 1000 Of proc1 Using termLTS. *)
 
-Example proc2 := tpar proc1 proc1.
-(* MeBi Show LTS Bounded 500 Of proc2 Using termLTS. *)
-(* MeBi Dump "proc2" LTS Bounded 500 Of proc2 Using termLTS. *)
+
+
+
+
 
 
 (* TODO: would be cool to do first a "FSM minimisation". I believe there are
@@ -258,33 +468,4 @@ Example proc2 := tpar proc1 proc1.
  completely irrelevant *)
 (* MeBi Show LTS Bounded 150 Of proc1 Using termLTS. *)
 (* MeBi Dump "proc0" FSM Bounded 150 Of proc1 Using termLTS. *)
-
-
-Inductive comp : Set :=
-| cterm : term -> comp
-| cpar : comp -> comp -> comp
-.
-
-(* second layer *)
-Inductive compLTS : comp -> bool -> comp -> Prop :=
-| do_t : forall a t t', termLTS t a t' -> compLTS (cterm t) a (cterm t')
-
-| do_l : forall a l l' r, compLTS l a l' -> compLTS (cpar l r) a (cpar l' r)
-| do_r : forall a l r r', compLTS r a r' -> compLTS (cpar l r) a (cpar l r')
-
-| do_l_end : forall a r, compLTS (cpar (cterm tend) r) a r
-| do_r_end : forall a l, compLTS (cpar l (cterm tend)) a l
-.
-
-Example comp0 := cpar (cterm proc1_rec1) (cterm proc1_rec1).
-(* MeBi Show LTS Bounded 150 Of comp0 Using termLTS compLTS. *)
-(* MeBi Dump "comp0" LTS Bounded 350 Of comp0 Using termLTS compLTS. *)
-
-Example comp1a := cpar (cterm proc1) (cterm tend).
-(* MeBi Show LTS Bounded 150 Of comp1a Using termLTS compLTS. *)
-(* MeBi Dump "comp1a" LTS Bounded 350 Of comp1a Using termLTS compLTS. *)
-
-Example comp1b := cpar (cterm proc1) (cterm proc1).
-(* MeBi Show LTS Bounded 150 Of comp1b Using termLTS compLTS. *)
-(* MeBi Dump "comp1b" LTS Bounded 5000 Of comp1b Using termLTS compLTS. *)
 
